tweak resultSet; prove stubbornness; not yet Lemma 7

Gossip/Error/SyncCorrection.lean
@@ -2,6 +2,8 @@ import Mathlib.Data.Set.Basic
 import Mathlib.Data.Prod.Basic
 import Mathlib.Tactic.Linarith
 
+namespace Error
+
 /-! # Synchronous One-Error Gossip with Correction -/
 
 /-! ## Basics
@@ -16,12 +18,8 @@ abbrev Value := (Agent × Bool) -- using Bool instead of 0 and 1
 -- We allow to write "a" for "(a, 1)", meaning NOT "(a, 0)" as in paper at the moment.
 instance : Coe Agent Value := ⟨fun a => ⟨a,true⟩⟩
 
-/-- (Def 1) Secret distribution -/
-abbrev Dist := Agent → Set Value
-
-/-- Every agent only has their own value. -/
-def isInitial (ι : Dist) :=
-  ∀ a, ι a = { ⟨a,True⟩ } ∨ ι a = { ⟨a,False⟩ }
+/-- An *initial* secret distribution, each agent only has their own value. -/
+abbrev Dist := Agent → Bool
 
 inductive Call : Type
   | normal : (caller : Agent) → (callee : Agent) → Call -- a b
@@ -51,7 +49,7 @@ instance {a : Agent} {c : Call} : Decidable (a ∈ c) := by
     try exact instDecidableTrue
     try exact instDecidableFalse
 
-/-- (Def 2) Call sequence.
+/-- (Def 2) A sequence of calls.
 For easier pattern matching this is in *reverse* order, i.e. the newest call is the first element. -/
 abbrev Sequence : Type := List Call
 
@@ -80,7 +78,7 @@ notation φ1:arg "⋀" φ2:arg => Con φ1 φ2
 notation φ1:arg "⋁" φ2:arg => Neg (Con (Neg φ1) (Neg φ2))
 notation φ1:arg "⟹" φ2:arg => (Neg φ1) ⋁ φ2
 
-notation "Kv" a:arg b:arg => (K a (S b b)) ⋁ (K a (S b (b,false)))
+notation "Kv" a:arg b:arg => (K a (S b (b, true))) ⋁ (K a (S b (b,false)))
 
 @[simp]
 def Form.length : Form → Nat
@@ -93,11 +91,13 @@ def Form.length : Form → Nat
 inductive Role : Type
   | Caller : Role
   | Callee : Role
+  /-- Not participating in the call -/
   | Other : Role
 deriving DecidableEq
 
 open Role
 
+/-- What is the `Role` of `i` in this call? -/
 def roleOfIn (i : Agent) : (c : Call) → Role
   | ⌜ a   b   ⌝ => if i = a then Caller else if i = b then Callee else Other
   | ⌜ a^_ b   ⌝ => if i = a then Caller else if i = b then Callee else Other
@@ -105,16 +105,27 @@ def roleOfIn (i : Agent) : (c : Call) → Role
 
 @[simp]
 lemma roleOfIn_a : roleOfIn a ⌜ a b ⌝ = Caller := by simp [roleOfIn]
+
+@[simp]
 lemma roleOfIn_eq_Caller_iff : roleOfIn a ⌜ x y ⌝ = Caller ↔ a = x := by simp [roleOfIn]; grind
+@[simp]
 lemma roleOfIn_eq_Callee_iff : roleOfIn a ⌜ x y ⌝ = Callee ↔ a ≠ x ∧ a = y := by simp [roleOfIn]; grind
+@[simp]
 lemma roleOfIn_eq_Other_iff : roleOfIn a ⌜ x y ⌝ = Other ↔ a ≠ x ∧ a ≠ y := by simp [roleOfIn]; grind
 
-/- TODO same lemmas for error calls?
-  | ⌜ a^_ b   ⌝ => if i = a then Caller else if i = b then Callee else Other
-  | ⌜ a   b^_ ⌝ => if i = a then Caller else if i = b then Callee else Other
--/
+@[simp]
+lemma roleOfIn_fstE_eq_Caller_iff : roleOfIn a ⌜ x^z y ⌝ = Caller ↔ a = x := by simp [roleOfIn]; grind
+@[simp]
+lemma roleOfIn_fstE_eq_Callee_iff : roleOfIn a ⌜ x^z y ⌝ = Callee ↔ a ≠ x ∧ a = y := by simp [roleOfIn]; grind
+@[simp]
+lemma roleOfIn_fstE_eq_Other_iff : roleOfIn a ⌜ x^z y ⌝ = Other ↔ a ≠ x ∧ a ≠ y := by simp [roleOfIn]; grind
 
-
+@[simp]
+lemma roleOfIn_sndE_eq_Caller_iff : roleOfIn a ⌜ x y^z ⌝ = Caller ↔ a = x := by simp [roleOfIn]; grind
+@[simp]
+lemma roleOfIn_sndE_eq_Callee_iff : roleOfIn a ⌜ x y^z ⌝ = Callee ↔ a ≠ x ∧ a = y := by simp [roleOfIn]; grind
+@[simp]
+lemma roleOfIn_sndE_eq_Other_iff : roleOfIn a ⌜ x y^z ⌝ = Other ↔ a ≠ x ∧ a ≠ y := by simp [roleOfIn]; grind
 
 /-! ## Semantics -/
 
@@ -122,26 +133,23 @@ mutual
 
 /-- (Def 4) Semantics of call.
 What values does this agent have after this sequence? -/
-def resultSet (a : Agent) : Dist → Sequence → Set Value
-  | ι, [] => ι a -- for the basis, ι[ε] = ι
+def resultSet (i : Agent) : Dist → Sequence → Set Value
+  | ι, [] => { (i, ι i) } -- for the basis, ι[ε] = ι
   | ι, (C :: σ) =>
-    let old := resultSet a ι σ
-    let knownIncorrect k : Set Value := fun v => -- the set *
-      match v with
-        | ⟨j,true ⟩ => eval ι σ (K k (S j (j,false)))
-        | ⟨j,false⟩ => eval ι σ (K k (S j (j,true )))
-    match C, roleOfIn a C with
+    /- (*) Which values did `i` already know to be wrong at state (ι,σ)? -/
+    let rejected : Set Value := { ⟨j, b⟩ | eval ι σ (K i (S j (j, !b))) }
+    match C, roleOfIn i C with
       -- Not involved:
-      | _, Other => old
-      -- Normal calls:
-      | ⌜ a b ⌝, Caller => (resultSet a ι σ) ∪ (resultSet b ι σ \ knownIncorrect b)
-      | ⌜ a b ⌝, Callee => (resultSet a ι σ \ knownIncorrect a) ∪ (resultSet b ι σ)
+      | _, Other => resultSet i ι σ
+       -- Normal calls
+      | ⌜ a b ⌝, Caller => (resultSet a ι σ ∪ resultSet b ι σ) \ rejected
+      | ⌜ a b ⌝, Callee => (resultSet a ι σ ∪ resultSet b ι σ) \ rejected
       -- error from a:
-      | ⌜ a^_ b ⌝, Caller => (resultSet a ι σ) ∪ (resultSet b ι σ \ knownIncorrect b) -- no self-error!
-      | ⌜ a^c b ⌝, Callee => (invert c $ resultSet a ι σ \ knownIncorrect a) ∪ (resultSet b ι σ)
+      | ⌜ a^_ b ⌝, Caller => (resultSet a ι σ ∪ resultSet b ι σ) \ rejected -- no self-error!
+      | ⌜ a^c b ⌝, Callee => (invert c (resultSet a ι σ) ∪ (resultSet b ι σ)) \ rejected
       -- error from b:
-      | ⌜ a b^c ⌝, Caller => (resultSet a ι σ) ∪ (invert c $ resultSet b ι σ \ knownIncorrect b)
-      | ⌜ a b^_ ⌝, Callee => (resultSet a ι σ \ knownIncorrect a) ∪ (resultSet b ι σ) -- no self-error!
+      | ⌜ a b^c ⌝, Caller => (resultSet a ι σ ∪ (invert c $ (resultSet b ι σ))) \ rejected
+      | ⌜ a b^_ ⌝, Callee => (resultSet a ι σ ∪ resultSet b ι σ) \ rejected -- no self-error!
 termination_by
   _ σ => (σ.length, 0) -- should be below contribSet
 decreasing_by
@@ -161,12 +169,13 @@ decreasing_by
 
 /-- (Def 5) Observation relation.
 This is *synchronous*. -/
-def equiv {k} (a : Agent) : (Dist × {σ : Sequence // σ.length = k}) → (Dist × {σ : Sequence // σ.length = k}) → Prop
-  | (ι, ⟨[]    ,_⟩), (ι', ⟨[]    ,_⟩) => isInitial ι ∧ isInitial ι' ∧ ι a = ι' a
+def equiv {k} (a : Agent) :
+    (Dist × {σ : Sequence // σ.length = k}) → (Dist × {σ : Sequence // σ.length = k}) → Prop
+  | (ι, ⟨[]    ,_⟩), (ι', ⟨[]    ,_⟩) => ι a = ι' a
   | (ι, ⟨C :: σ,_⟩), (ι', ⟨D :: τ,_⟩) =>
                           @equiv (k-1) a (ι,⟨σ, by aesop⟩) (ι',⟨τ, by aesop⟩)
                         ∧ roleOfIn a C = roleOfIn a D
-                        -- Depending on the role, observe who is in the call and the contribSet of the other
+                        -- Depending on role, observe (contribSet of) the other agent in the call
                         ∧ match roleOfIn a C with
                           | Other => True
                           | Caller => (contribSet ι σ C).2 = (contribSet ι' τ D).2 ∧ C.pair = D.pair
@@ -186,10 +195,7 @@ decreasing_by
 def eval : Dist → Sequence → Form → Prop
   | _, _, .Top => True
   | ι, σ, .Neg φ => ¬ eval ι σ φ
-  | ι, σ, .S a (j, k) =>
-      if a == j
-      then (j, k) ∈ ι a -- Here we hard-code stubbornness :-)
-      else (j, k) ∈ resultSet a ι σ
+  | ι, σ, .S a (j, k) => (j, k) ∈ resultSet a ι σ
   | ι, σ, .Con φ ψ => eval ι σ φ ∧ eval ι σ ψ
   | ι, σ, .K a φ => ∀ t, ∀ τ , (he : equiv a (ι,⟨σ,rfl⟩) (t,τ)) → eval t τ φ
 termination_by
@@ -208,22 +214,136 @@ end
 
 notation ι:arg "⌈" σ:arg "⌉" a:arg => resultSet a ι σ
 
+@[simp]
+lemma resultSet_nil {ι i} : resultSet i ι []  = { (i, ι i) } := by simp [resultSet]
+
+@[simp]
+lemma equiv_nil : equiv i (ι, ⟨[],h1⟩) (κ, ⟨[],h2⟩) ↔ ι i = κ i := by simp [equiv]
+
+/-! ## Notation and Abbreviations -/
+
+notation ισ:100 "⊧" φ:100 => eval ισ.1 ισ.2 φ
+
 /-- An abbreviation to easily say that we have the same length and (can thus say) `equiv`. -/
 def equi (a : Agent) (ισ : Dist × Sequence) (ι'τ : Dist × Sequence) : Prop :=
   ∃ h : ισ.2.length = ι'τ.2.length, equiv a ⟨ισ.1, ⟨ισ.2, rfl⟩⟩ ⟨ι'τ.1, ⟨ι'τ.2, h.symm⟩⟩
 
 notation ισ:arg " ~_ " a:arg ι'τ:arg => equi a ισ ι'τ
 
-notation ισ "⊧" φ => eval ισ.1 ισ.2 φ
-
 /-- Validity of formulas -/
 def valid (φ : Form) := ∀ ι σ, eval ι σ φ
+
 prefix:100 "⊨" => valid -- FIXME what's a good precedence value here?
 
-lemma same_set_then_know_same (same_set : ι⌈σ'⌉b = ι'⌈τ'⌉b) :
-    eval ι' τ' (K b (S a (a, v))) ↔ eval ι σ' (K b (S a (a, v))) := by
-  sorry
+/-! ## Properties of the Semantics -/
 
+lemma equiv_refl : equiv (a : Agent) (ι, σ) (ι, σ) := by
+  unfold equiv
+  split
+  · simp_all
+  case h_2 he1 he2 =>
+    simp_all
+    rcases he1 with ⟨_,_,_⟩
+    rcases he2 with ⟨_,_⟩
+    subst_eqs
+    simp
+    cases roleOfIn a _ <;> simp_all <;> apply equiv_refl
+
+/-- Agents know their own initial state. -/
+lemma true_of_knowldege {ι σ a φ} :
+    eval ι σ (K a φ) → eval ι σ φ := by
+  intro hyp
+  simp [eval] at hyp
+  exact hyp ι σ rfl equiv_refl
+
+/-- Agents know their own initial state. -/
+lemma know_self n σ τ (h1 : σ.length = n) (h2 : τ.length = n) :
+    equiv a (ι, ⟨σ, h1⟩) (κ, ⟨τ, h2⟩) → ι a = κ a  := by
+  induction n generalizing ι κ σ τ
+  · rw [List.length_eq_zero_iff] at h1
+    rw [List.length_eq_zero_iff] at h2
+    subst h1 h2
+    simp
+  case succ n IH =>
+    rcases List.exists_cons_of_length_eq_add_one h1 with ⟨c1, σ, σ_def⟩
+    rcases List.exists_cons_of_length_eq_add_one h2 with ⟨c2, τ, τ_def⟩
+    unfold equiv
+    cases h : roleOfIn a c1 <;> aesop
+
+/-- Agents are stubborn about their own secrets. -/
+lemma stubbornness n σ (h : σ.length = n) :
+    eval ι σ (S a (a, k)) ↔ ι a = k := by
+  simp [eval]
+  induction n generalizing σ k ι
+  case zero =>
+    rw [List.length_eq_zero_iff] at h
+    subst h
+    simp
+    grind
+  case succ n IH =>
+    rcases List.exists_cons_of_length_eq_add_one h with ⟨c, σ, σ_def⟩
+    subst σ_def
+    unfold resultSet
+    simp
+    cases rh : roleOfIn a c <;> cases c <;> simp <;> simp at h
+    any_goals -- Caller
+      simp at rh
+      subst rh
+      constructor
+      · rintro ⟨(ak_in|ak_in), not_k⟩
+        · rw [IH _ h] at ak_in; assumption
+        · simp [eval] at not_k
+          rcases not_k with ⟨κ, τ, ⟨same, equ⟩, not_in⟩
+          have := know_self _ _ _ _ _ equ
+          specialize @IH κ (!k) τ (by grind)
+          aesop
+      · intro ak_in
+        constructor
+        · left
+          rw [IH _ h]
+          assumption
+        · intro hyp
+          simp [eval] at hyp
+          specialize hyp ι σ rfl equiv_refl
+          grind
+    any_goals -- Callee
+      simp at rh
+      rcases rh with ⟨rh1,rh2⟩
+      subst rh2
+      constructor
+      · rintro ⟨(ak_in|ak_in), not_k⟩
+        · simp [eval] at not_k
+          rcases not_k with ⟨κ, τ, ⟨same, equ⟩, not_in⟩
+          have := know_self _ _ _ _ _ equ
+          specialize @IH κ (!k) τ (by grind)
+          aesop
+        · rw [IH _ h] at ak_in; assumption
+      · intro ak_in
+        constructor
+        · right
+          rw [IH _ h]
+          assumption
+        · intro hyp
+          simp [eval] at hyp
+          specialize hyp ι σ rfl equiv_refl
+          grind
+    any_goals -- Other, easy
+      simp at rh
+      rcases rh with ⟨rh1,rh2⟩
+      rw [IH _ h]
+
+lemma same_set_then_know_same
+    (same_set : ι⌈σ'⌉b = ι'⌈τ'⌉b) (same_len : σ'.length = τ'.length)
+    : eval ι' τ' (K b (S a (a, v))) ↔ eval ι σ' (K b (S a (a, v))) := by
+  unfold eval
+  simp
+  simp_rw [stubbornness]
+  constructor
+  · intro hyp κ ρ same_len equ
+    specialize hyp κ ρ (by aesop)
+    -- is this actually true???
+    sorry
+  · sorry
 
 /-- Lemma 7 -/
 lemma indistinguishable_then_same_values {ι ι': Dist} {σ τ : Sequence} :
@@ -233,8 +353,7 @@ lemma indistinguishable_then_same_values {ι ι': Dist} {σ τ : Sequence} :
   induction σ generalizing τ
   case nil =>
     have := List.length_eq_zero_iff.mp same_len.symm
-    subst this
-    simp_all [resultSet, equiv]
+    aesop
   case cons κ σ' IH =>
     simp at same_len
     rcases List.exists_cons_of_length_eq_add_one same_len.symm with ⟨κ', τ', τ_def⟩
@@ -247,15 +366,14 @@ lemma indistinguishable_then_same_values {ι ι': Dist} {σ τ : Sequence} :
       simp [r] at equ
       rcases equ with ⟨prev_equ, Caller_eq, prev_same_contrib, same_pair⟩
       unfold contribSet at prev_same_contrib
-      cases κ <;> cases κ' <;> simp at * -- 6 cases should drop out here?
-      case normal.normal a_ b a__ b__ =>
-        rw [roleOfIn_eq_Caller_iff] at r
-        subst r
-        rw [Eq.comm, roleOfIn_eq_Caller_iff] at Caller_eq
-        subst Caller_eq
-        simp [Call.pair] at same_pair
-        subst same_pair
+      cases κ <;> cases κ' <;> simp [Call.pair, roleOfIn_eq_Caller_iff] at *
+      all_goals
+        rcases same_pair with ⟨_,_⟩
+        subst_eqs
+      -- 6 cases should drop out here?
+      case normal.normal =>
         simp at same_len
+        clear Caller_eq -- useless?
         unfold resultSet
         simp
         ext x
@@ -265,15 +383,17 @@ lemma indistinguishable_then_same_values {ι ι': Dist} {σ τ : Sequence} :
           · aesop
           · aesop
           · rcases x with ⟨v,b⟩
-            cases b <;> simp [Set.instMembership, Set.Mem]
+            cases b <;> simp
             all_goals
-              rw [same_set_then_know_same]; tauto
+              rw [same_set_then_know_same] <;> tauto
         · intro hyp; convert hyp using 2
           · aesop
           · rcases x with ⟨v,b⟩
             cases b <;> simp [Set.instMembership, Set.Mem]
             all_goals
-              rw [same_set_then_know_same]; tauto
+              sorry
+              -- rw [same_set_then_know_same] <;> tauto
+          · sorry -- via extra lemma equiv_trans etc?
       all_goals
         -- 8 more cases ... can we do this in a more general helper lemma?
         sorry
@@ -318,3 +438,5 @@ Examples?
 /-- Proposition 17, 18 and 19 maybe too hard? -/
 
 -/
+
+end Error
