Gossip.lean
@@ -2,3 +2,4 @@ import Gossip.Basic
 import Gossip.Sufficient
 import Gossip.Necessary
 import Gossip.Evaluation
+import Gossip.Error.SyncCorrection
